Make implementations stateful

examples/miniparse/MiniParse.Impl.Int.fst
@@ -3,6 +3,21 @@ include MiniParse.Spec.Int
 include MiniParse.Impl.Combinators
 
 module U8 = FStar.UInt8
-module B32 = MiniParse.Bytes32
+module B = LowStar.Buffer
+module U32 = FStar.UInt32
+module HST = FStar.HyperStack.ST
 
-let parse32_u8 : parser32 parse_u8 = make_total_constant_size_parser32 1 1ul (fun x -> Seq.index x 0) () (fun x -> B32.get x 0ul)
+let parse32_u8 : parser32 parse_u8 = make_total_constant_size_parser32 1 1ul (fun x -> Seq.index x 0) () (fun x -> B.index x 0ul)
+
+let serialize32_u8 : serializer32 serialize_u8 =
+  (fun output (len: U32.t { len == B.len output } ) x ->
+    let h = HST.get () in
+    if len `U32.lt` 1ul
+    then None
+    else begin
+      let output' = B.sub output 0ul 1ul in
+      B.upd output' 0ul x;
+      let h' = HST.get () in
+      assert (B.as_seq h' output' `Seq.equal` Seq.create 1 x);
+      Some 1ul
+    end)
